Rename various mem and stack types to machine_heap, vale_heap, etc.

vale/code/arch/x64/Vale.X64.Decls.fsti
@@ -13,6 +13,7 @@ open Vale.X64.Machine_s
 open Vale.X64.State
 open Vale.Def.Types_s
 
+unfold let vale_heap = M.vale_heap
 unfold let quad32 = quad32
 
 val cf : (flags:int) -> bool
@@ -75,46 +76,46 @@ val mul_nat_helper (x y:nat) : Lemma (x `op_Multiply` y >= 0)
 
 (* Abbreviations *)
 unfold let get_reg (o:va_reg_operand) : reg = Reg 0 (OReg?.r o)
-unfold let buffer_readable (#t:M.base_typ) (h:M.mem) (b:M.buffer t) : GTot prop0 = M.buffer_readable #t h b
+unfold let buffer_readable (#t:M.base_typ) (h:vale_heap) (b:M.buffer t) : GTot prop0 = M.buffer_readable #t h b
 unfold let buffer_writeable (#t:M.base_typ) (b:M.buffer t) : GTot prop0 = M.buffer_writeable #t b
 unfold let buffer_length (#t:M.base_typ) (b:M.buffer t) = M.buffer_length #t b
-unfold let buffer8_as_seq (m:M.mem) (b:M.buffer8) : GTot (Seq.seq nat8) = M.buffer_as_seq m b
-unfold let buffer64_as_seq (m:M.mem) (b:M.buffer64) : GTot (Seq.seq nat64) = M.buffer_as_seq m b
-unfold let s64 (m:M.mem) (b:M.buffer64) : GTot (Seq.seq nat64) = buffer64_as_seq m b
-unfold let buffer128_as_seq (m:M.mem) (b:M.buffer128) : GTot (Seq.seq quad32) = M.buffer_as_seq m b
-unfold let s128 (m:M.mem) (b:M.buffer128) : GTot (Seq.seq quad32) = buffer128_as_seq m b
-unfold let valid_src_addr (#t:M.base_typ) (m:M.mem) (b:M.buffer t) (i:int) : prop0 =
+unfold let buffer8_as_seq (m:vale_heap) (b:M.buffer8) : GTot (Seq.seq nat8) = M.buffer_as_seq m b
+unfold let buffer64_as_seq (m:vale_heap) (b:M.buffer64) : GTot (Seq.seq nat64) = M.buffer_as_seq m b
+unfold let s64 (m:vale_heap) (b:M.buffer64) : GTot (Seq.seq nat64) = buffer64_as_seq m b
+unfold let buffer128_as_seq (m:vale_heap) (b:M.buffer128) : GTot (Seq.seq quad32) = M.buffer_as_seq m b
+unfold let s128 (m:vale_heap) (b:M.buffer128) : GTot (Seq.seq quad32) = buffer128_as_seq m b
+unfold let valid_src_addr (#t:M.base_typ) (m:vale_heap) (b:M.buffer t) (i:int) : prop0 =
   0 <= i /\ i < buffer_length b /\ buffer_readable m b
-unfold let valid_dst_addr (#t:M.base_typ) (m:M.mem) (b:M.buffer t) (i:int) : prop0 =
+unfold let valid_dst_addr (#t:M.base_typ) (m:vale_heap) (b:M.buffer t) (i:int) : prop0 =
   0 <= i /\ i < buffer_length b /\ buffer_readable m b /\ buffer_writeable b
-unfold let buffer64_read (b:M.buffer64) (i:int) (m:M.mem) : GTot nat64 = M.buffer_read b i m
-unfold let buffer64_write (b:M.buffer64) (i:int) (v:nat64) (m:M.mem) : GTot M.mem =
+unfold let buffer64_read (b:M.buffer64) (i:int) (m:vale_heap) : GTot nat64 = M.buffer_read b i m
+unfold let buffer64_write (b:M.buffer64) (i:int) (v:nat64) (m:vale_heap) : GTot vale_heap =
   if FStar.StrongExcludedMiddle.strong_excluded_middle (buffer_readable m b /\ buffer_writeable b) then
     M.buffer_write b i v m else m
-unfold let buffer128_read (b:M.buffer128) (i:int) (m:M.mem) : GTot quad32 = M.buffer_read b i m
-unfold let buffer128_write (b:M.buffer128) (i:int) (v:quad32) (m:M.mem) : GTot M.mem =
+unfold let buffer128_read (b:M.buffer128) (i:int) (m:vale_heap) : GTot quad32 = M.buffer_read b i m
+unfold let buffer128_write (b:M.buffer128) (i:int) (v:quad32) (m:vale_heap) : GTot vale_heap =
   if FStar.StrongExcludedMiddle.strong_excluded_middle (buffer_readable m b /\ buffer_writeable b) then
     M.buffer_write b i v m else m
-unfold let modifies_mem (s:M.loc) (h1 h2:M.mem) : GTot prop0 = M.modifies s h1 h2
+unfold let modifies_mem (s:M.loc) (h1 h2:vale_heap) : GTot prop0 = M.modifies s h1 h2
 unfold let loc_buffer(#t:M.base_typ) (b:M.buffer t) = M.loc_buffer #t b
 unfold let locs_disjoint = M.locs_disjoint
 unfold let loc_union = M.loc_union
 
-let valid_maddr (addr:int) (s_mem:M.mem) (s_memTaint:M.memtaint) (b:M.buffer64) (index:int) (t:taint) : prop0 =
+let valid_maddr (addr:int) (s_mem:vale_heap) (s_memTaint:M.memtaint) (b:M.buffer64) (index:int) (t:taint) : prop0 =
   valid_src_addr s_mem b index /\
   M.valid_taint_buf64 b s_mem s_memTaint t /\
   addr == M.buffer_addr b s_mem + 8 `op_Multiply` index
 
-let valid_maddr128 (addr:int) (s_mem:M.mem) (s_memTaint:M.memtaint) (b:M.buffer128) (index:int) (t:taint) : prop0 =
+let valid_maddr128 (addr:int) (s_mem:vale_heap) (s_memTaint:M.memtaint) (b:M.buffer128) (index:int) (t:taint) : prop0 =
   valid_src_addr s_mem b index /\
   M.valid_taint_buf128 b s_mem s_memTaint t /\
   addr == M.buffer_addr b s_mem + 16 `op_Multiply` index
 
-let valid_mem_operand (addr:int) (t:taint) (s_mem:M.mem) (s_memTaint:M.memtaint) : prop0 =
+let valid_mem_operand (addr:int) (t:taint) (s_mem:vale_heap) (s_memTaint:M.memtaint) : prop0 =
   exists (b:M.buffer64) (index:int).{:pattern (valid_maddr addr s_mem s_memTaint b index t)}
     valid_maddr addr s_mem s_memTaint b index t
 
-let valid_mem_operand128 (addr:int) (t:taint) (s_mem:M.mem) (s_memTaint:M.memtaint) : prop0 =
+let valid_mem_operand128 (addr:int) (t:taint) (s_mem:vale_heap) (s_memTaint:M.memtaint) : prop0 =
   exists (b:M.buffer128) (index:int).{:pattern (valid_maddr128 addr s_mem s_memTaint b index t)}
     valid_maddr128 addr s_mem s_memTaint b index t
 
@@ -122,7 +123,7 @@ let valid_mem_operand128 (addr:int) (t:taint) (s_mem:M.mem) (s_memTaint:M.memtai
 let valid_operand (o:operand64) (s:vale_state) : prop0 =
   Vale.X64.State.valid_src_operand o s /\
   ( match o with
-    | OMem (m, t) -> valid_mem_operand (eval_maddr m s) t s.vs_mem s.vs_memTaint
+    | OMem (m, t) -> valid_mem_operand (eval_maddr m s) t s.vs_heap s.vs_memTaint
     | OStack (m, t) -> S.valid_taint_stack64 (eval_maddr m s) t s.vs_stackTaint
     | _ -> True
   )
@@ -131,7 +132,7 @@ let valid_operand (o:operand64) (s:vale_state) : prop0 =
 let valid_operand128 (o:operand128) (s:vale_state) : prop0 =
   Vale.X64.State.valid_src_operand128 o s /\
   ( match o with
-    | OMem (m, t) -> valid_mem_operand128 (eval_maddr m s) t s.vs_mem s.vs_memTaint
+    | OMem (m, t) -> valid_mem_operand128 (eval_maddr m s) t s.vs_heap s.vs_memTaint
     | OStack (m, t) -> S.valid_taint_stack128 (eval_maddr m s) t s.vs_stackTaint
     | _ -> True
   )
@@ -180,13 +181,13 @@ unfold let va_opr_code_Mem (o:va_operand) (offset:int) (t:taint) : va_operand =
 val va_opr_lemma_Mem (s:va_state) (base:va_operand) (offset:int) (b:M.buffer64) (index:int) (t:taint) : Lemma
   (requires
     OReg? base /\
-    valid_src_addr s.vs_mem b index /\
-    M.valid_taint_buf64 b s.vs_mem s.vs_memTaint t /\
-    eval_operand base s + offset == M.buffer_addr b s.vs_mem + 8 `op_Multiply` index
+    valid_src_addr s.vs_heap b index /\
+    M.valid_taint_buf64 b s.vs_heap s.vs_memTaint t /\
+    eval_operand base s + offset == M.buffer_addr b s.vs_heap + 8 `op_Multiply` index
   )
   (ensures
     valid_operand (va_opr_code_Mem base offset t) s /\
-    M.load_mem64 (M.buffer_addr b s.vs_mem + 8 `op_Multiply` index) s.vs_mem == M.buffer_read b index s.vs_mem
+    M.load_mem64 (M.buffer_addr b s.vs_heap + 8 `op_Multiply` index) s.vs_heap == M.buffer_read b index s.vs_heap
   )
 
 [@va_qattr]
@@ -212,13 +213,13 @@ unfold let va_opr_code_Mem128 (o:va_operand) (offset:int) (t:taint) : va_operand
 val va_opr_lemma_Mem128 (s:va_state) (base:va_operand) (offset:int) (t:taint) (b:M.buffer128) (index:int) : Lemma
   (requires
     OReg? base /\
-    valid_src_addr s.vs_mem b index /\
-    M.valid_taint_buf128 b s.vs_mem s.vs_memTaint t /\
-    eval_operand base s + offset == M.buffer_addr b s.vs_mem + 16 `op_Multiply` index
+    valid_src_addr s.vs_heap b index /\
+    M.valid_taint_buf128 b s.vs_heap s.vs_memTaint t /\
+    eval_operand base s + offset == M.buffer_addr b s.vs_heap + 16 `op_Multiply` index
   )
   (ensures
     valid_operand128 (va_opr_code_Mem128 base offset t) s /\
-    M.load_mem128 (M.buffer_addr b s.vs_mem + 16 `op_Multiply` index) s.vs_mem == M.buffer_read b index s.vs_mem
+    M.load_mem128 (M.buffer_addr b s.vs_heap + 16 `op_Multiply` index) s.vs_heap == M.buffer_read b index s.vs_heap
   )
 
 val taint_at (memTaint:M.memtaint) (addr:int) : taint
@@ -252,8 +253,8 @@ val taint_at (memTaint:M.memtaint) (addr:int) : taint
 [@va_qattr] unfold let va_get_flags (s:va_state) : int = s.vs_flags
 [@va_qattr] unfold let va_get_reg (r:reg_64) (s:va_state) : nat64 = eval_reg_64 r s
 [@va_qattr] unfold let va_get_xmm (x:reg_xmm) (s:va_state) : quad32 = eval_reg_xmm x s
-[@va_qattr] unfold let va_get_mem (s:va_state) : M.mem = s.vs_mem
-[@va_qattr] unfold let va_get_stack (s:va_state) : S.stack = s.vs_stack
+[@va_qattr] unfold let va_get_mem (s:va_state) : vale_heap = s.vs_heap
+[@va_qattr] unfold let va_get_stack (s:va_state) : S.vale_stack = s.vs_stack
 [@va_qattr] unfold let va_get_memTaint (s:va_state) : M.memtaint = s.vs_memTaint
 [@va_qattr] unfold let va_get_stackTaint (s:va_state) : M.memtaint = s.vs_stackTaint
 
@@ -262,8 +263,8 @@ val taint_at (memTaint:M.memtaint) (addr:int) : taint
 //[@va_qattr] let va_upd_reg (r:reg) (v:t_reg r) (s:vale_state) : vale_state = update_reg r v s
 [@va_qattr] let va_upd_reg (r:reg_64) (v:nat64) (s:vale_state) : vale_state = update_reg_64 r v s
 [@va_qattr] let va_upd_xmm (x:reg_xmm) (v:quad32) (s:vale_state) : vale_state = update_reg_xmm x v s
-[@va_qattr] let va_upd_mem (mem:M.mem) (s:vale_state) : vale_state = { s with vs_mem = mem }
-[@va_qattr] let va_upd_stack (stack:S.stack) (s:vale_state) : vale_state = { s with vs_stack = stack }
+[@va_qattr] let va_upd_mem (mem:vale_heap) (s:vale_state) : vale_state = { s with vs_heap = mem }
+[@va_qattr] let va_upd_stack (stack:S.vale_stack) (s:vale_state) : vale_state = { s with vs_stack = stack }
 [@va_qattr] let va_upd_memTaint (memTaint:M.memtaint) (s:vale_state) : vale_state = { s with vs_memTaint = memTaint }
 [@va_qattr] let va_upd_stackTaint (stackTaint:M.memtaint) (s:vale_state) : vale_state = { s with vs_stackTaint = stackTaint }
 
@@ -277,7 +278,7 @@ val taint_at (memTaint:M.memtaint) (addr:int) : taint
   va_upd_reg r (eval_reg_64 r sM) sK
 [@va_qattr] unfold let va_update_xmm (x:reg_xmm) (sM:va_state) (sK:va_state) : va_state =
   va_upd_xmm x (eval_reg_xmm x sM) sK
-[@va_qattr] unfold let va_update_mem (sM:va_state) (sK:va_state) : va_state = va_upd_mem sM.vs_mem sK
+[@va_qattr] unfold let va_update_mem (sM:va_state) (sK:va_state) : va_state = va_upd_mem sM.vs_heap sK
 [@va_qattr] unfold let va_update_stack (sM:va_state) (sK:va_state) : va_state = va_upd_stack sM.vs_stack sK
 [@va_qattr] unfold let va_update_memTaint (sM:va_state) (sK:va_state) : va_state = va_upd_memTaint sM.vs_memTaint sK
 [@va_qattr] unfold let va_update_stackTaint (sM:va_state) (sK:va_state) : va_state = va_upd_stackTaint sM.vs_stackTaint sK
@@ -372,7 +373,7 @@ unfold let va_get_whileBody (c:va_code{While? c}) : va_code = While?.whileBody c
 
 (** Map syntax **)
 
-//unfold let op_String_Access (m:M.mem) (b:M.buffer64) = fun index -> buffer64_read b index m
+//unfold let op_String_Access (m:vale_heap) (b:M.buffer64) = fun index -> buffer64_read b index m
 
 // syntax for map accesses, m.[key] and m.[key] <- value
 (*
@@ -398,59 +399,59 @@ let memModified (old_mem:mem) (new_mem:mem) (ptr:int) (num_bytes) =
 *)
 
 (** Convenient memory-related functions **)
-let rec buffers_readable (h: M.mem) (l: list M.buffer64) : GTot prop0 (decreases l) =
+let rec buffers_readable (h: vale_heap) (l: list M.buffer64) : GTot prop0 (decreases l) =
     match l with
     | [] -> True
     | b :: l'  -> buffer_readable h b /\ buffers_readable h l'
 
-unfold let modifies_none (h1 h2:M.mem) = modifies_mem M.loc_none h1 h2
-unfold let modifies_buffer (b:M.buffer64) (h1 h2:M.mem) = modifies_mem (loc_buffer b) h1 h2
-unfold let modifies_buffer_2 (b1 b2:M.buffer64) (h1 h2:M.mem) =modifies_mem (M.loc_union (loc_buffer b1) (loc_buffer b2)) h1 h2
-unfold let modifies_buffer_3 (b1 b2 b3:M.buffer64) (h1 h2:M.mem) =modifies_mem (M.loc_union (M.loc_union (loc_buffer b1) (loc_buffer b2)) (loc_buffer b3)) h1 h2
-unfold let modifies_buffer128 (b:M.buffer128) (h1 h2:M.mem) = modifies_mem (loc_buffer b) h1 h2
-unfold let modifies_buffer128_2 (b1 b2:M.buffer128) (h1 h2:M.mem) = modifies_mem (M.loc_union (loc_buffer b1) (loc_buffer b2)) h1 h2
-unfold let modifies_buffer128_3 (b1 b2 b3:M.buffer128) (h1 h2:M.mem) = modifies_mem (M.loc_union (M.loc_union (loc_buffer b1) (loc_buffer b2)) (loc_buffer b3)) h1 h2
+unfold let modifies_none (h1 h2:vale_heap) = modifies_mem M.loc_none h1 h2
+unfold let modifies_buffer (b:M.buffer64) (h1 h2:vale_heap) = modifies_mem (loc_buffer b) h1 h2
+unfold let modifies_buffer_2 (b1 b2:M.buffer64) (h1 h2:vale_heap) =modifies_mem (M.loc_union (loc_buffer b1) (loc_buffer b2)) h1 h2
+unfold let modifies_buffer_3 (b1 b2 b3:M.buffer64) (h1 h2:vale_heap) =modifies_mem (M.loc_union (M.loc_union (loc_buffer b1) (loc_buffer b2)) (loc_buffer b3)) h1 h2
+unfold let modifies_buffer128 (b:M.buffer128) (h1 h2:vale_heap) = modifies_mem (loc_buffer b) h1 h2
+unfold let modifies_buffer128_2 (b1 b2:M.buffer128) (h1 h2:vale_heap) = modifies_mem (M.loc_union (loc_buffer b1) (loc_buffer b2)) h1 h2
+unfold let modifies_buffer128_3 (b1 b2 b3:M.buffer128) (h1 h2:vale_heap) = modifies_mem (M.loc_union (M.loc_union (loc_buffer b1) (loc_buffer b2)) (loc_buffer b3)) h1 h2
 
-let validSrcAddrs64 (m:M.mem) (addr:int) (b:M.buffer64) (len:int) (memTaint:M.memtaint) (t:taint) =
+let validSrcAddrs64 (m:vale_heap) (addr:int) (b:M.buffer64) (len:int) (memTaint:M.memtaint) (t:taint) =
     buffer_readable m b /\
     len <= buffer_length b /\
     M.buffer_addr b m == addr /\
     M.valid_taint_buf64 b m memTaint t
 
-let validDstAddrs64 (m:M.mem) (addr:int) (b:M.buffer64) (len:int) (memTaint:M.memtaint) (t:taint) =
+let validDstAddrs64 (m:vale_heap) (addr:int) (b:M.buffer64) (len:int) (memTaint:M.memtaint) (t:taint) =
     buffer_readable m b /\
     buffer_writeable b /\
     len <= buffer_length b /\
     M.buffer_addr b m == addr /\
     M.valid_taint_buf64 b m memTaint t
 
-let validSrcAddrs128 (m:M.mem) (addr:int) (b:M.buffer128) (len:int) (memTaint:M.memtaint) (t:taint) =
+let validSrcAddrs128 (m:vale_heap) (addr:int) (b:M.buffer128) (len:int) (memTaint:M.memtaint) (t:taint) =
     buffer_readable m b /\
     len <= buffer_length b /\
     M.buffer_addr b m == addr /\
     M.valid_taint_buf128 b m memTaint t
 
-let validDstAddrs128 (m:M.mem) (addr:int) (b:M.buffer128) (len:int) (memTaint:M.memtaint) (t:taint) =
+let validDstAddrs128 (m:vale_heap) (addr:int) (b:M.buffer128) (len:int) (memTaint:M.memtaint) (t:taint) =
     buffer_readable m b /\
     buffer_writeable b /\
     len <= buffer_length b /\
     M.buffer_addr b m == addr /\
     M.valid_taint_buf128 b m memTaint t
 
-let validSrcAddrsOffset128 (m:M.mem) (addr:int) (b:M.buffer128) (offset len:int) (memTaint:M.memtaint) (t:taint) =
+let validSrcAddrsOffset128 (m:vale_heap) (addr:int) (b:M.buffer128) (offset len:int) (memTaint:M.memtaint) (t:taint) =
     buffer_readable m b /\
     offset + len <= buffer_length b /\
     M.buffer_addr b m + 16 `op_Multiply` offset == addr /\
     M.valid_taint_buf128 b m memTaint t
 
-let validDstAddrsOffset128 (m:M.mem) (addr:int) (b:M.buffer128) (offset len:int) (memTaint:M.memtaint) (t:taint) =
+let validDstAddrsOffset128 (m:vale_heap) (addr:int) (b:M.buffer128) (offset len:int) (memTaint:M.memtaint) (t:taint) =
     buffer_readable m b /\
     buffer_writeable b /\
     offset + len <= buffer_length b /\
     M.buffer_addr b m + 16 `op_Multiply` offset == addr /\
     M.valid_taint_buf128 b m memTaint t
 
-let modifies_buffer_specific128 (b:M.buffer128) (h1 h2:M.mem) (start last:nat) : GTot prop0 =
+let modifies_buffer_specific128 (b:M.buffer128) (h1 h2:vale_heap) (start last:nat) : GTot prop0 =
     modifies_buffer128 b h1 h2 /\
     // TODO: Consider replacing this with: modifies (loc_buffer (gsub_buffer b i len)) h1 h2
     (forall (i:nat) . {:pattern (Seq.index (M.buffer_as_seq h2 b) i)}
@@ -459,7 +460,7 @@ let modifies_buffer_specific128 (b:M.buffer128) (h1 h2:M.mem) (start last:nat) :
                     ==> buffer128_read b i h1
                      == buffer128_read b i h2)
 
-let buffer_modifies_specific128 (b:M.buffer128) (h1 h2:M.mem) (start last:nat) : GTot prop0 =
+let buffer_modifies_specific128 (b:M.buffer128) (h1 h2:vale_heap) (start last:nat) : GTot prop0 =
     // TODO: Consider replacing this with: modifies (loc_buffer (gsub_buffer b i len)) h1 h2
     (forall (i:nat) . {:pattern (Seq.index (M.buffer_as_seq h2 b) i)}
                         0 <= i /\ i < buffer_length b
@@ -467,7 +468,7 @@ let buffer_modifies_specific128 (b:M.buffer128) (h1 h2:M.mem) (start last:nat) :
                     ==> buffer128_read b i h1
                      == buffer128_read b i h2)
 
-let modifies_buffer_specific (b:M.buffer64) (h1 h2:M.mem) (start last:nat) : GTot prop0 =
+let modifies_buffer_specific (b:M.buffer64) (h1 h2:vale_heap) (start last:nat) : GTot prop0 =
     modifies_buffer b h1 h2 /\
     // TODO: Consider replacing this with: modifies (loc_buffer (gsub_buffer b i len)) h1 h2
     (forall (i:nat) . {:pattern (Seq.index (M.buffer_as_seq h2 b) i)}
