vale/code/arch/x64/Vale.X64.StateLemmas.fst
@@ -10,7 +10,7 @@ module F = FStar.FunctionalExtensionality
 
 #reset-options "--initial_fuel 2 --max_fuel 2"
 
-let same_domain sv s = MS.same_domain sv.vs_mem s.BS.ms_mem
+let same_domain sv s = MS.same_domain sv.vs_heap s.BS.ms_heap
 
 let same_domain_eval_ins c f s0 sv =
   match c with
@@ -18,14 +18,14 @@ let same_domain_eval_ins c f s0 sv =
     let obs = BS.ins_obs ins s0 in
     let s1 = {BS.machine_eval_ins ins ({s0 with BS.ms_trace = []}) with BS.ms_trace = obs @ s0.BS.ms_trace} in
     Vale.X64.Bytes_Semantics.eval_ins_domains ins ({s0 with BS.ms_trace = []});
-    MS.lemma_same_domains sv.vs_mem s0.BS.ms_mem s1.BS.ms_mem
+    MS.lemma_same_domains sv.vs_heap s0.BS.ms_heap s1.BS.ms_heap
 
 let state_to_S (s:vale_state) : GTot BS.machine_state =
   {
     BS.ms_ok = s.vs_ok;
     BS.ms_regs = F.on_dom reg (fun r -> Regs.sel r s.vs_regs);
     BS.ms_flags = int_to_nat64 s.vs_flags;
-    BS.ms_mem = MS.get_heap s.vs_mem;
+    BS.ms_heap = MS.get_heap s.vs_heap;
     BS.ms_memTaint = s.vs_memTaint;
     BS.ms_stack = VSS.stack_to_s s.vs_stack;
     BS.ms_stackTaint = s.vs_stackTaint;
@@ -33,12 +33,12 @@ let state_to_S (s:vale_state) : GTot BS.machine_state =
   }
 
 let state_of_S (sv:vale_state) (s:BS.machine_state{same_domain sv s}) : GTot vale_state =
-  let { BS.ms_ok = ok; BS.ms_regs = regs; BS.ms_flags = flags; BS.ms_mem = mem; BS.ms_stack = stack} = s in
+  let { BS.ms_ok = ok; BS.ms_regs = regs; BS.ms_flags = flags; BS.ms_heap = mem; BS.ms_stack = stack} = s in
   {
     vs_ok = ok;
     vs_regs = Regs.of_fun regs;
     vs_flags = flags;
-    vs_mem = MS.get_hs sv.vs_mem mem;
+    vs_heap = MS.get_hs sv.vs_heap mem;
     vs_memTaint = s.BS.ms_memTaint;
     vs_stack = VSS.stack_from_s stack;
     vs_stackTaint = s.BS.ms_stackTaint;
@@ -61,7 +61,7 @@ let lemma_to_eval_operand s o =
   | OConst _ | OReg _ -> ()
   | OMem (m, _) ->
     let addr = eval_maddr m s in
-    MS.equiv_load_mem addr s.vs_mem
+    MS.equiv_load_mem addr s.vs_heap
   | OStack (m, _) -> ()
 
 #reset-options "--initial_fuel 2 --max_fuel 2"
@@ -74,7 +74,7 @@ let lemma_to_eval_operand128 s o =
   | OConst _ | OReg _ -> ()
   | OMem (m, _) ->
     let addr = eval_maddr m s in
-    MS.equiv_load_mem128 addr s.vs_mem
+    MS.equiv_load_mem128 addr s.vs_heap
   | OStack (m, _) -> ()
 
 #reset-options "--initial_fuel 2 --max_fuel 2"
@@ -86,7 +86,7 @@ let lemma_to_valid_operand s o =
     let aux () : Lemma
       (requires valid_src_operand o s)
       (ensures BS.valid_src_operand o (state_to_S s)) =
-      MS.bytes_valid addr s.vs_mem
+      MS.bytes_valid addr s.vs_heap
       in
     Classical.move_requires aux ()
   | OStack (m, _) -> ()
@@ -104,17 +104,17 @@ let lemma_to_of_eval_ins c s0 =
   same_domain_eval_ins c 0 s0' s0;
   let s' = state_of_S s0 sM in
   let s'' = state_to_S s' in
-  let {BS.ms_ok = ok; BS.ms_regs = regs; BS.ms_flags = flags; BS.ms_mem = heap; BS.ms_stack = stack} = sM in
-  let {BS.ms_ok = ok''; BS.ms_regs = regs''; BS.ms_flags = flags''; BS.ms_mem = heap''; BS.ms_stack = stack''} = s'' in
+  let {BS.ms_ok = ok; BS.ms_regs = regs; BS.ms_flags = flags; BS.ms_heap = heap; BS.ms_stack = stack} = sM in
+  let {BS.ms_ok = ok''; BS.ms_regs = regs''; BS.ms_flags = flags''; BS.ms_heap = heap''; BS.ms_stack = stack''} = s'' in
   assert (feq regs regs'');
   Vale.X64.Bytes_Semantics.eval_ins_same_unspecified ins s0';
   Vale.X64.Bytes_Semantics.eval_ins_domains ins s0';
   VSS.lemma_stack_to_from stack;
-  MS.get_heap_hs heap s0.vs_mem
+  MS.get_heap_hs heap s0.vs_heap
 
 val lemma_valid_taint64: (b:ME.buffer64) ->
                          (memTaint:ME.memtaint) ->
-                         (mem:ME.mem) ->
+                         (mem:ME.vale_heap) ->
                          (i:nat{i < ME.buffer_length b}) ->
                          (t:taint) -> Lemma
   (requires ME.valid_taint_buf64 b mem memTaint t /\ ME.buffer_readable mem b)
@@ -122,7 +122,7 @@ val lemma_valid_taint64: (b:ME.buffer64) ->
 
 val lemma_valid_taint128: (b:ME.buffer128) ->
                          (memTaint:ME.memtaint) ->
-                         (mem:ME.mem) ->
+                         (mem:ME.vale_heap) ->
                          (i:nat{i < ME.buffer_length b}) ->
                          (t:taint) -> Lemma
   (requires ME.valid_taint_buf128 b mem memTaint t /\ ME.buffer_readable mem b)
@@ -131,8 +131,8 @@ val lemma_valid_taint128: (b:ME.buffer128) ->
 
 
 val same_memTaint64: (b:ME.buffer64) ->
-                   (mem0:ME.mem) ->
-                   (mem1:ME.mem) ->
+                   (mem0:ME.vale_heap) ->
+                   (mem1:ME.vale_heap) ->
                    (memtaint0:ME.memtaint) ->
                    (memtaint1:ME.memtaint) -> Lemma
   (requires (ME.modifies (ME.loc_buffer b) mem0 mem1 /\
@@ -140,8 +140,8 @@ val same_memTaint64: (b:ME.buffer64) ->
   (ensures memtaint0 == memtaint1)
 
 val same_memTaint128: (b:ME.buffer128) ->
-                   (mem0:ME.mem) ->
-                   (mem1:ME.mem) ->
+                   (mem0:ME.vale_heap) ->
+                   (mem1:ME.vale_heap) ->
                    (memtaint0:ME.memtaint) ->
                    (memtaint1:ME.memtaint) -> Lemma
   (requires (ME.modifies (ME.loc_buffer b) mem0 mem1 /\
