vale/code/arch/x64/interop/Vale.X64.MemoryAdapters.fsti
@@ -12,27 +12,27 @@ module V = Vale.X64.Decls
 val as_vale_buffer (#src #t:_) (i:IB.buf_t src t) : GTot (ME.buffer t)
 val as_vale_immbuffer (#src #t:_) (i:IB.ibuf_t src t) : GTot (ME.buffer t)
 
-val mem_eq : squash (ME.mem == IB.mem)
-val stack_eq : squash (BS.stack == SI.stack)
+val mem_eq : squash (ME.vale_heap == IB.interop_heap)
+val stack_eq : squash (BS.machine_stack == SI.vale_stack)
 
 unfold
-let as_mem (m:ME.mem)
-  : IB.mem
+let as_mem (m:ME.vale_heap)
+  : IB.interop_heap
   = IB.coerce m
 
 unfold
-let as_vale_mem (m:IB.mem)
-  : ME.mem
+let as_vale_mem (m:IB.interop_heap)
+  : ME.vale_heap
   = IB.coerce m
 
 unfold
-let as_vale_stack (st:BS.stack)
-  : SI.stack
+let as_vale_stack (st:BS.machine_stack)
+  : SI.vale_stack
   = IB.coerce st
 
 val buffer_addr_is_nat64 (#t:_) (x:ME.buffer t) (s:VS.vale_state)
-  : Lemma (0 <= ME.buffer_addr x VS.(s.vs_mem) /\
-           ME.buffer_addr x VS.(s.vs_mem) < pow2 64)
+  : Lemma (0 <= ME.buffer_addr x VS.(s.vs_heap) /\
+           ME.buffer_addr x VS.(s.vs_heap) < pow2 64)
 
 val code_equiv : squash (V.va_code == Vale.X64.Machine_Semantics_s.code)
 val ins_equiv : squash (V.ins == Vale.X64.Machine_Semantics_s.ins)
