vale/code/crypto/poly1305/x64/Vale.Poly1305.Util.fsti
@@ -37,27 +37,27 @@ let seqTo128 (s:Seq.seq nat64) : t_seqTo128 =
   in f
 let seqTo128_app (s:Seq.seq nat64) (i:int) : nat128 = seqTo128 s i
 
-val lemma_poly1305_heap_hash_blocks_alt (h:int) (pad:int) (r:int) (m:mem) (b:buffer64) (n:int) : Lemma
+val lemma_poly1305_heap_hash_blocks_alt (h:int) (pad:int) (r:int) (m:vale_heap) (b:buffer64) (n:int) : Lemma
   (requires 0 <= n /\ n + n <= buffer_length b /\ n + n <= Seq.length (buffer64_as_seq m b))
   (ensures
     ((n + n) % 2) == 0 /\ // REVIEW
     poly1305_heap_blocks h pad r (buffer64_as_seq m b) (n + n) ==
     poly1305_hash_blocks h pad r (seqTo128 (buffer64_as_seq m b)) n)
 
-let rec buffers_readable (h:mem) (l:list buffer64) : GTot Type0 (decreases l) =
+let rec buffers_readable (h:vale_heap) (l:list buffer64) : GTot Type0 (decreases l) =
   match l with
   | [] -> True
   | b :: l'  -> buffer_readable h b /\ buffers_readable h l'
 
-unfold let modifies_buffer (b:buffer64) (h1 h2:mem) = modifies_mem (loc_buffer b) h1 h2
+unfold let modifies_buffer (b:buffer64) (h1 h2:vale_heap) = modifies_mem (loc_buffer b) h1 h2
 
-let validSrcAddrs64 (m:mem) (addr:int) (b:buffer64) (len:int) (memTaint:memtaint) (t:taint) =
+let validSrcAddrs64 (m:vale_heap) (addr:int) (b:buffer64) (len:int) (memTaint:memtaint) (t:taint) =
   buffer_readable m b /\
   len <= buffer_length b /\
   buffer_addr b m == addr /\
   valid_taint_buf64 b m memTaint t
 
-let modifies_buffer_specific (b:buffer64) (h1 h2:mem) (start last:nat) : GTot prop0 =
+let modifies_buffer_specific (b:buffer64) (h1 h2:vale_heap) (start last:nat) : GTot prop0 =
   modifies_buffer b h1 h2 /\
   (forall (i:nat).{:pattern (Seq.index (buffer_as_seq h2 b) i)}
     0 <= i /\ i < buffer_length b /\ (i < start || i > last) ==>
