vale/specs/hardware/Vale.X64.Leakage_s.fst
@@ -25,26 +25,26 @@ let publicRegisterValuesAreSame (ts:analysis_taints) (s1:machine_state) (s2:mach
     (s1.ms_regs r = s2.ms_regs r)
 
 let publicMemValueIsSame
-  (mem1 mem2:heap)
+  (mem1 mem2:machine_heap)
   (memTaint1 memTaint2:Map.t int taint)
   (x:int) =
   (Public? (memTaint1.[x]) || Public? (memTaint2.[x])) ==>
      mem1.[x] == mem2.[x]
 
 let publicMemValuesAreSame (s1:machine_state) (s2:machine_state) =
-  forall x.{:pattern s1.ms_memTaint.[x] \/ s2.ms_memTaint.[x] \/ s1.ms_mem.[x] \/ s2.ms_mem.[x]}
-    publicMemValueIsSame s1.ms_mem s2.ms_mem s1.ms_memTaint s2.ms_memTaint x
+  forall x.{:pattern s1.ms_memTaint.[x] \/ s2.ms_memTaint.[x] \/ s1.ms_heap.[x] \/ s2.ms_heap.[x]}
+    publicMemValueIsSame s1.ms_heap s2.ms_heap s1.ms_memTaint s2.ms_memTaint x
 
 let publicStackValueIsSame
-  (stack1 stack2:heap)
+  (stack1 stack2:machine_heap)
   (stackTaint1 stackTaint2:Map.t int taint)
   (x:int)
   = (Public? (stackTaint1.[x]) || Public? (stackTaint2.[x])) ==>
      stack1.[x] == stack2.[x]
 
 let publicStackValuesAreSame (s1:machine_state) (s2:machine_state) =
-  let Vale_stack _ stack1 = s1.ms_stack in
-  let Vale_stack _ stack2 = s2.ms_stack in
+  let Machine_stack _ stack1 = s1.ms_stack in
+  let Machine_stack _ stack2 = s2.ms_stack in
   forall x.{:pattern s1.ms_stackTaint.[x] \/ s2.ms_stackTaint.[x] \/ stack1.[x] \/ stack2.[x]}
     publicStackValueIsSame stack1 stack2 s1.ms_stackTaint s2.ms_stackTaint x
 
